coq/theories/imp2asm/CompilerProofs.v
@@ -9,48 +9,27 @@ From impboot.derivations Require Import CompilerDerivations.
 From impboot.imp2asm Require Import ImpToASMCodegenProofs.
 From impboot.fp2imp Require Import FpToImpCodegenProof.
 
-(* forall input prog output1 output2,
-    prog_terminates input prog fuel output1 sd /\
-    asm_terminates input (codegen prog) sd output2 ->
-      output1 = output2. *)
-
-(* 
-Theorem compiler_asm_correct:
-  ∀input output.
-    (input, compiler_asm) asm_terminates output ⇒
-    output = compiler input
-Proof
-  metis_tac [compiler_asm_def,codegen_terminates,compiler_prog_correct]
-QED
-
-Theorem compiler_compiler_str:
-  compiler compiler_str = compiler_asm_str
-Proof
-  fs [compiler_str_def,codegenTheory.compiler_def,
-      parser_lexer_prog2str,compiler_asm_str_def,compiler_asm_def]
-QED
-
-Theorem compiler_asm_bootstrap:
-  (compiler_str, compiler_asm) asm_terminates output ⇒
-  output = compiler_asm_str
-Proof
-  metis_tac [compiler_asm_correct,compiler_compiler_str]
-QED
-*)
-
-Theorem compiler_correct: forall input output sd,
-  asm_terminates (Llist.of_list input) compiler_program_asm sd output ->
+Theorem compiler_correct: forall input output,
+  asm_terminates (Llist.of_list input) compiler_program_asm output ->
   output = compiler input.
 Proof.
   intros * Hasm_terminates.
   specialize (compiler_program_thm input) as Hfp_compiler_thm.
   specialize compiler_program_imp_exists as [compiler_imp Hcompiler_program_imp]; subst.
   unfold compiler_program_imp in *.
+  Opaque compiler FpToImpCodegen.to_imp ImpToASMCodegen.codegen.
   eapply to_imp_thm in Hfp_compiler_thm; eauto.
   unfold ImpSemantics.imp_weak_termination in *; cleanup.
-  eapply codegen_terminates with (output2 := compiler input).
-Admitted.
+  unfold compiler_program_asm, compiler_program_imp in *; rewrite Hcompiler_program_imp in *.
+  symmetry; eapply codegen_terminates with (input := Llist.of_list input) (prog := compiler_imp).
+  split; [|eauto].
+  unfold ImpSemantics.prog_terminates; do 2 eexists.
+  split; [eauto|].
+  eapply H1.
+  eapply codegen_no_abort; eauto.
+Qed.
 
+Transparent compiler FpToImpCodegen.to_imp ImpToASMCodegen.codegen.
 Theorem print_parser_compiler_correct:
   match compiler_program_imp with
   | None => False
@@ -61,9 +40,18 @@ Proof.
   lazy; reflexivity.
 Qed.
 
-(* TODO: move to Bootstrapping.v? *)
-Eval lazy in (match compiler_program_imp with
-  | None => ""
-  | Some compiler_imp =>
-    imp2str compiler_imp
-  end).
+Theorem compiler_asm_bootstrap: forall output,
+  asm_terminates (Llist.of_list (list_ascii_of_string compiler_imp_str)) compiler_program_asm output ->
+  output = compiler_asm_str.
+Proof.
+  intros * Hasm_terminates.
+  unfold compiler_imp_str in *.
+  unfold compiler_asm_str, compiler_program_asm.
+  specialize print_parser_compiler_correct as Hprint_parser_compiler_correct.
+  specialize compiler_program_imp_exists as [compiler_imp Hcompiler_program_imp]; rewrite Hcompiler_program_imp in *.
+  eapply compiler_correct in Hasm_terminates; eauto; rewrite Hasm_terminates.
+  unfold compiler, dlet.
+  rewrite <- Hprint_parser_compiler_correct in *.
+  reflexivity.
+  Opaque FpToImpCodegen.to_imp ImpToASMCodegen.codegen.
+Qed.
